src/crypto/loopunroll/testreturnvalue.c
@@ -1,0 +1,36 @@
+/*
+  Test code for returning a value from a value procedure.
+  Brian Milnes, 25 Sept 2017.
+
+  Both Linux and 
+
+*/
+#include <stdlib.h>
+#include <stdio.h>
+#include <stdint.h> // for uint?_t
+#include <string.h> // for memcmp
+#include <ctype.h> // for memcmp
+#include "gcc_compat.h" // For registers.
+
+int __stdcall ReturnValue1();
+int __stdcall ReturnValue0();
+
+void test_return_value() {
+// According to the ABI we put the value in RAX.
+  int r1 = ReturnValue1();
+  if (r1 == 1) {
+  } else {
+    printf("Expecting 1 got %d FAILED\n", r1);
+  }
+  int r0 = ReturnValue0();
+  if (r0 == 0) {
+  } else {
+    printf("Expecting 0 got %d FAILED\n", r0);
+  }
+}
+
+void __cdecl main(void) {
+  printf("Test return value from Vale\n");
+  test_return_value();
+  printf("Test return value from Vale Finished.\n");
+}
